examples/test/test.fst
@@ -1,8 +1,47 @@
 module Test
 
-(* let f (x:int) : int = 0 *)
+type rw =
+  | Reader
+  | Writer
 
-(* val f : int -> Tot int *)
-let f x =
-  let rec aux : int -> Tot int = fun x -> aux x in
-  aux 0
+new type id
+new type rid
+new type rref : rid -> Type0 -> Type0
+new type entry : id -> Type0
+new type seq : Type0 -> Type0
+
+type state (i:id) (rw:rw) =
+  | State: #region:rid 
+         -> #peer_region:rid
+         -> log: rref (if rw=Reader then peer_region else region) (seq (entry i)) // ghost, subject to cryptographic assumption
+         -> state i rw
+
+type writer i = s:state i Writer
+type reader i = s:state i Reader
+
+// Generate a fresh instance with index i in a fresh sub-region of r0
+// (we might drop this spec, since F* will infer something at least as precise,
+// but we keep it for documentation)
+val gen: reader_parent:rid -> writer_parent:rid -> i:id -> ST (reader i * writer i)
+  (requires (fun h0 -> HyperHeap.disjoint reader_parent writer_parent))
+  (ensures  (fun h0 (rw:reader i * writer i) h1 ->
+           let r = fst rw in 
+           let w = snd rw in 
+           (* let bang = fun x -> sel h1 x in  *)
+           modifies Set.empty h0 h1
+         /\ w.region = r.peer_region
+         /\ r.region = w.peer_region
+         /\ extends (w.region) writer_parent
+         /\ extends (r.region) reader_parent
+         /\ fresh_region w.region h0 h1
+         /\ fresh_region r.region h0 h1
+         /\ op_Equality #(rref w.region (seq (entry i))) w.log r.log  //the explicit annotation here 
+         /\ contains_ref w.counter h1
+         /\ contains_ref r.counter h1
+         /\ contains_ref w.log h1
+         /\ sel h1 w.counter = 0
+         /\ sel h1 r.counter = 0
+         /\ sel h1 w.log = createEmpty
+         ))
+
+
